src/program_proof/tulip/program/gcoord/gpreparer_repr.v
@@ -198,12 +198,11 @@ Section repr.
       "Hgpp" ∷ own_gpreparer_with_phase gpp phase ts gid γ.
 
   Definition own_gpreparer_uninit (gpp : loc) : iProp Σ :=
-    ∃ (nrps : u64) (phase : u64) (frespmP : loc) (vdmP : loc) (srespmP : loc),
-      "HnrpsP"   ∷ gpp ↦[GroupPreparer :: "nrps"] #nrps ∗
+    ∃ (phase : u64) (frespmP : loc) (vdmP : loc) (srespmP : loc),
       "HphaseP"  ∷ gpp ↦[GroupPreparer :: "phase"] #phase ∗
       "HfrespmP" ∷ gpp ↦[GroupPreparer :: "frespm"] #frespmP ∗
       "HvdmP"    ∷ gpp ↦[GroupPreparer :: "vdm"] #vdmP ∗
       "HsrespmP" ∷ gpp ↦[GroupPreparer :: "srespm"] #srespmP ∗
-      "%Hnrps"   ∷ ⌜uint.nat nrps = size rids_all⌝.
+      "Hnrps"    ∷ own_gpreparer_nrps gpp.
 
 End repr.
