src/program_proof/tulip/program/gcoord/gpreparer_attach.v
@@ -1,0 +1,42 @@
+From Perennial.program_proof.tulip.program Require Import prelude.
+From Perennial.program_proof.tulip.program.gcoord Require Import gpreparer_repr.
+  
+Section program.
+  Context `{!heapGS Σ, !tulip_ghostG Σ}.
+
+  Theorem wp_GroupPreparer__attach (gpp : loc) ts gid γ :
+    {{{ own_gpreparer_uninit gpp ∗ own_txn_client_token γ ts gid }}}
+      GroupPreparer__attach #gpp
+    {{{ RET #(); own_gpreparer gpp ts gid γ }}}.
+  Proof.
+    iIntros (Φ) "[Hgpp Hcli] HΦ".
+    wp_rec.
+
+    (*@ func (gpp *GroupPreparer) reset() {                                     @*)
+    (*@     gpp.phase = GPP_VALIDATING                                          @*)
+    (*@     gpp.frespm = make(map[uint64]bool)                                  @*)
+    (*@     gpp.vdm = make(map[uint64]bool)                                     @*)
+    (*@ }                                                                       @*)
+    iNamed "Hgpp".
+    wp_storeField.
+    wp_apply (wp_NewMap u64 bool).
+    iIntros (frespmP') "Hfrespm".
+    wp_storeField.
+    wp_apply (wp_NewMap u64 bool).
+    iIntros (vdmP') "Hvdm".
+    wp_storeField.
+    iApply "HΦ".
+    iFrame "HphaseP HfrespmP HvdmP HsrespmP ∗ %".
+    iExists GPPValidating. simpl.
+    iModIntro.
+    iSplit; first done.
+    iSplit.
+    { iSplit; last done. by iApply big_sepM_empty. }
+    iSplit.
+    { iSplit; last done. by rewrite /validation_responses dom_empty_L big_sepS_empty. }
+    iSplit.
+    { iExists ∅. done. }
+    by iFrame.
+  Qed.
+
+End program.
