src/program_proof/tulip/program/gcoord/mk_gcoord.v
@@ -1,68 +1,22 @@
 From Perennial.program_proof.tulip.program Require Import prelude.
 From Perennial.program_proof.tulip.program.gcoord Require Import
-  gpreparer_repr greader_repr gcoord_repr.
+  gcoord_repr mk_greader mk_gpreparer.
   
 Section program.
   Context `{!heapGS Σ, !tulip_ghostG Σ}.
 
-  Theorem wp_GroupPreparer__reset (gpp : loc) ts gid γ :
-    {{{ own_gpreparer_uninit gpp }}}
-      GroupPreparer__reset #gpp
-    {{{ RET #(); own_gpreparer gpp ts gid γ }}}.
-  Proof.
-    iIntros (Φ) "Hgpp HΦ".
-    wp_rec.
-
-    (*@ func (gpp *GroupPreparer) reset() {                                     @*)
-    (*@     gpp.phase = GPP_VALIDATING                                          @*)
-    (*@     gpp.frespm = make(map[uint64]bool)                                  @*)
-    (*@     gpp.vdm = make(map[uint64]bool)                                     @*)
-    (*@ }                                                                       @*)
-    iNamed "Hgpp".
-    wp_storeField.
-    wp_apply (wp_NewMap u64 bool).
-    iIntros (frespmP') "Hfrespm".
-    wp_storeField.
-    wp_apply (wp_NewMap u64 bool).
-    iIntros (vdmP') "Hvdm".
-    wp_storeField.
-    iApply "HΦ".
-    iFrame "HnrpsP HphaseP HfrespmP HvdmP HsrespmP ∗ %".
-    iExists GPPValidating. simpl.
-    iModIntro.
-    iSplit; first done.
-    iSplit.
-    { iSplit; last done. by iApply big_sepM_empty. }
-    iSplit.
-    { iSplit; last done. by rewrite /validation_responses dom_empty_L big_sepS_empty. }
-    iSplit.
-    { iExists ∅. done. }
-    
-    rewrite Hnrps.
-    simpl.
-    iSplit
-  Admitted.
-
-  Theorem wp_mkGroupPreparer (nrps : u64) gid γ :
-    {{{ True }}}
-      mkGroupPreparer #nrps
-    {{{ (gpp : loc), RET #gpp; own_gpreparer gpp O gid γ }}}.
-  Proof.
-    (*@ func mkGroupPreparer(nrps uint64) *GroupPreparer {                      @*)
-    (*@     gpp := &GroupPreparer{ nrps : nrps }                                @*)
-    (*@     gpp.reset()                                                         @*)
-    (*@                                                                         @*)
-    (*@     return gpp                                                          @*)
-    (*@ }                                                                       @*)
-  Admitted.
-
   Theorem wp_mkGroupCoordinator (addrmP : loc) (addrm : gmap u64 chan) gid γ :
+    gid ∈ gids_all ->
+    dom addrm = rids_all ->
     own_map addrmP DfracDiscarded addrm -∗
+    know_tulip_inv γ -∗
+    know_tulip_network_inv γ gid addrm -∗
     {{{ True }}}
       mkGroupCoordinator #addrmP
-    {{{ (gcoord : loc), RET #gcoord; is_gcoord gcoord gid γ }}}.
+    {{{ (gcoord : loc), RET #gcoord; is_gcoord_with_addrm gcoord gid addrm γ }}}.
   Proof.
-    iIntros "#Haddrm" (Φ) "!> _ HΦ".
+    iIntros (Hgid Hdomaddrm) "#Haddrm #Hinv #Hinvnet".
+    iIntros (Φ) "!> _ HΦ".
     wp_rec.
 
     (*@ func mkGroupCoordinator(addrm map[uint64]grove_ffi.Address) *GroupCoordinator { @*)
@@ -93,9 +47,10 @@ Section program.
     set P := (λ (mx : gmap u64 chan), ∃ (rpsP' : Slice.t) (l : list u64),
                  "HrpsP" ∷ rpsPP ↦[slice.T uint64T] rpsP' ∗
                  "Hrps"  ∷ own_slice rpsP' uint64T (DfracOwn 1) l ∗
-                 "%Hrps" ∷ ⌜list_to_set l = dom mx⌝)%I.
+                 "%Hrps" ∷ ⌜list_to_set l = dom mx⌝ ∗
+                 "%Hnd"  ∷ ⌜NoDup l⌝)%I.
     wp_apply (wp_MapIter_fold _ _ _ P with "Haddrm [$Hrps $HrpsP]").
-    { done. }
+    { by rewrite NoDup_nil. }
     { clear Φ.
       iIntros (mx rid c Φ) "!> [HP %Hrid] HΦ".
       iNamed "HP".
@@ -107,6 +62,11 @@ Section program.
       iFrame.
       iPureIntro.
       rewrite list_to_set_app_L dom_insert_L Hrps /=.
+      split; first set_solver.
+      apply NoDup_snoc; last done.
+      destruct Hrid as [Hnotin _].
+      apply not_elem_of_dom in Hnotin.
+      rewrite -Hrps in Hnotin.
       set_solver.
     }
     iIntros "[_ HP]".
@@ -126,10 +86,54 @@ Section program.
     (*@     }                                                                   @*)
     (*@                                                                         @*)
     wp_load.
+    wp_apply (wp_mkGroupReader).
+    { rewrite -Hdomaddrm size_dom. word. }
+    iIntros (grd) "Hgrd".
+    wp_apply (wp_mkGroupPreparer).
+    { rewrite -Hdomaddrm size_dom. word. }
+    iIntros (gpp) "Hgpp".
+    wp_apply (wp_NewMap u64 bool).
+    iIntros (tsfinalsP) "Htsfinals".
+    wp_apply (map.wp_NewMap).
+    iIntros (conns) "Hconns".
+    rewrite {1}/zero_val /=.
+    wp_pures.
+    wp_apply (wp_allocStruct).
+    { by auto 15. }
+    iIntros (gcoord) "Hgcoord".
+    iDestruct (struct_fields_split with "Hgcoord") as "Hgcoord".
+    iNamed "Hgcoord".
+    wp_pures.
 
     (*@     return gcoord                                                       @*)
     (*@ }                                                                       @*)
-  Admitted.
-
+    iApply "HΦ".
+    iAssert (own_gcoord_ts gcoord O)%I with "[$ts]" as "Hts"; first word.
+    iAssert (own_gcoord_greader gcoord O γ)%I with "[$grd $Hgrd]" as "Hgrd".
+    iAssert (own_gcoord_gpreparer gcoord O gid γ)%I with "[$gpp $Hgpp]" as "Hgpp".
+    iAssert (own_gcoord_finalizer gcoord (dom addrm))%I
+      with "[$idxleader $tsfinals $Htsfinals]" as "Hfinalizer".
+    { rewrite Hdomaddrm size_rids_all. word. }
+    iAssert (own_gcoord_core gcoord O gid (dom addrm) γ)%I
+      with "[$Hts $Hgrd $Hgpp $Hfinalizer]" as "Hgcoord".
+    iAssert (own_gcoord_comm gcoord addrm gid γ)%I with "[$conns Hconns]" as "Hcomm".
+    { iExists ∅.
+      rewrite fmap_empty big_sepM_empty.
+      by iFrame.
+    }
+    iAssert (own_gcoord gcoord addrm gid γ)%I with "[$Hgcoord $Hcomm]" as "Hgcoord".
+    iMod (alloc_lock _ _ _ (own_gcoord gcoord addrm gid γ) with "Hfree [$Hgcoord]") as "#Hlock".
+    iMod (readonly_alloc_1 with "mu") as "#HmuP".
+    iMod (readonly_alloc_1 with "cv") as "#HcvP".
+    iMod (readonly_alloc_1 with "cvrs") as "#HcvrsP".
+    iClear "HrpsP".
+    iMod (readonly_alloc_1 with "rps") as "#HrpsP".
+    iMod (readonly_alloc_1 with "addrm") as "#HaddrmP".
+    iDestruct (own_slice_to_small with "Hrps") as "Hrps".
+    iMod (readonly_alloc_1 with "Hrps") as "#Hrps".
+    iFrame "# %".
+    iPureIntro.
+    by rewrite Hrps.
+  Qed.
 
 End program.
