src/program_proof/tulip/program/gcoord/mk_gpreparer.v
@@ -1,0 +1,51 @@
+From Perennial.program_proof.tulip.program Require Import prelude.
+From Perennial.program_proof.tulip.program.gcoord Require Import gpreparer_repr .
+  
+Section program.
+  Context `{!heapGS Σ, !tulip_ghostG Σ}.
+
+  Theorem wp_mkGroupPreparer (nrps : u64) gid γ :
+    uint.nat nrps = size rids_all ->
+    {{{ True }}}
+      mkGroupPreparer #nrps
+    {{{ (gpp : loc), RET #gpp; own_gpreparer gpp O gid γ }}}.
+  Proof.
+    iIntros (Hnrps Φ) "_ HΦ".
+    wp_rec.
+
+    (*@ func mkGroupPreparer(nrps uint64) *GroupPreparer {                      @*)
+    (*@     gpp := &GroupPreparer{ nrps : nrps }                                @*)
+    (*@     gpp.phase = GPP_WAITING                                             @*)
+    (*@     gpp.frespm = make(map[uint64]bool)                                  @*)
+    (*@     gpp.vdm = make(map[uint64]bool)                                     @*)
+    (*@                                                                         @*)
+    wp_apply (wp_allocStruct).
+    { by auto 10. }
+    iIntros (gpp) "Hgpp".
+    iDestruct (struct_fields_split with "Hgpp") as "Hgpp".
+    iNamed "Hgpp".
+    wp_storeField.
+    wp_apply (wp_NewMap u64 bool).
+    iIntros (frespmP) "Hfrespm".
+    wp_storeField.
+    wp_apply (wp_NewMap u64 bool).
+    iIntros (vdmP) "Hvdm".
+    wp_storeField.
+    
+    (*@     return gpp                                                          @*)
+    (*@ }                                                                       @*)
+    iApply "HΦ".
+    iFrame "nrps phase frespm vdm srespm ∗ %".
+    iExists GPPWaiting.
+    iModIntro.
+    iSplit; first done.
+    iSplit.
+    { iSplit; last done. by iApply big_sepM_empty. }
+    iSplit.
+    { iSplit; last done. by rewrite /validation_responses dom_empty_L big_sepS_empty. }
+    iSplit.
+    { iExists ∅. done. }
+    by iFrame.
+  Qed.
+
+End program.
