src/program_proof/tulip/program/gcoord/mk_greader.v
@@ -1,0 +1,36 @@
+From Perennial.program_proof.tulip.program Require Import prelude.
+From Perennial.program_proof.tulip.program.gcoord Require Import
+  greader_repr greader_reset.
+  
+Section program.
+  Context `{!heapGS Σ, !tulip_ghostG Σ}.
+
+  Theorem wp_mkGroupReader (nrps : u64) γ :
+    uint.nat nrps = size rids_all ->
+    {{{ True }}}
+      mkGroupReader #nrps
+    {{{ (grd : loc), RET #grd; own_greader grd O γ }}}.
+  Proof.
+    iIntros (Hrid Φ) "_ HΦ".
+    wp_rec.
+
+    (*@ func mkGroupReader(nrps uint64) *GroupReader {                          @*)
+    (*@     grd := &GroupReader{ nrps : nrps }                                  @*)
+    (*@     grd.reset()                                                         @*)
+    (*@     return grd                                                          @*)
+    (*@ }                                                                       @*)
+    wp_apply (wp_allocStruct).
+    { by auto 10. }
+    iIntros (grd) "Hgrd".
+    wp_pures.
+    wp_apply (wp_GroupReader__reset with "[Hgrd]").
+    { iDestruct (struct_fields_split with "Hgrd") as "Hgrd".
+      iNamed "Hgrd".
+      by iFrame.
+    }
+    iIntros "Hgrd".
+    wp_pures.
+    by iApply "HΦ".
+  Qed.
+
+End program.
