src/program_proof/tulip/program/gcoord/start.v
@@ -1,0 +1,65 @@
+From Perennial.program_proof.tulip.program Require Import prelude.
+From Perennial.program_proof.tulip.program.gcoord Require Import
+  gcoord_repr mk_gcoord gcoord_response_session gcoord_resend_session.
+From Goose.github_com.mit_pdos.tulip Require Export gcoord.
+  
+Section program.
+  Context `{!heapGS Σ, !tulip_ghostG Σ}.
+
+  Theorem wp_Start (addrmP : loc) (addrm : gmap u64 chan) gid γ :
+    gid ∈ gids_all ->
+    dom addrm = rids_all ->
+    own_map addrmP DfracDiscarded addrm -∗
+    know_tulip_inv γ -∗
+    know_tulip_network_inv γ gid addrm -∗
+    {{{ True }}}
+      Start #addrmP
+    {{{ (gcoord : loc), RET #gcoord; is_gcoord gcoord gid γ }}}.
+  Proof.
+    iIntros (Hgid Hdomaddrm) "#Haddrm #Hinv #Hinvnet".
+    iIntros (Φ) "!> _ HΦ".
+    wp_rec.
+
+    (*@ func Start(addrm map[uint64]grove_ffi.Address) *GroupCoordinator {      @*)
+    (*@     gcoord := mkGroupCoordinator(addrm)                                 @*)
+    (*@                                                                         @*)
+    wp_apply (wp_mkGroupCoordinator with "Haddrm Hinv Hinvnet").
+    { apply Hgid. }
+    { apply Hdomaddrm. }
+    iIntros (gcoord) "#Hgcoord".
+
+    (*@     for ridloop := range(addrm) {                                       @*)
+    (*@         rid := ridloop                                                  @*)
+    (*@         go func() {                                                     @*)
+    (*@             gcoord.ResponseSession(rid)                                 @*)
+    (*@         }()                                                             @*)
+    (*@     }                                                                   @*)
+    (*@                                                                         @*)
+    wp_apply (wp_MapIter_fold _ _ _ (λ _ : gmap u64 chan, True)%I with "Haddrm []"); first done.
+    { clear Φ.
+      iIntros (m rid addr Φ) "!> [_ [_ %Haddr]] HΦ".
+      wp_apply wp_fork; last by iApply "HΦ".
+      wp_apply (wp_GroupCoordinator__ResponseSession with "Hgcoord").
+      { apply Haddr. }
+      done.
+    }
+    iIntros "_".
+
+    (*@     go func() {                                                         @*)
+    (*@         gcoord.ResendSession()                                          @*)
+    (*@     }()                                                                 @*)
+    (*@                                                                         @*)
+    wp_apply wp_fork.
+    { wp_apply (wp_GroupCoordinator__ResendSession).
+      { by iFrame "Hgcoord". }
+      done.
+    }
+
+    (*@     return gcoord                                                       @*)
+    (*@ }                                                                       @*)
+    wp_pures.
+    iApply "HΦ".
+    by iFrame "Hgcoord".
+  Qed.
+
+End program.
